eval function to lists of values + tc function + mc function

multiplicities/multiplicities.v
@@ -1,39 +1,96 @@
+Require Import List.
+Import ListNotations.
+
+Fixpoint list_pair_with {X Y : Type} (lx : list X) (y : Y) : list (X*Y) :=
+  match lx with
+  | [] => []
+  | x :: tx => (x, y) :: (list_pair_with tx y)
+  end.
+
+Fixpoint list_pair_with2 {X Y : Type} (x : X) (ly : list Y) : list (X*Y) :=
+  match ly with
+  | [] => []
+  | y :: ty => (x, y) :: (list_pair_with2 x ty)
+  end.
+
+Fixpoint list_crossproduct {X Y : Type} (lx : list X) (ly : list Y) : list (X*Y) :=
+  match lx with
+  | [] => []
+  | x :: tx => (list_pair_with2 x ly) ++ (list_crossproduct tx ly)
+  end.
+
+(***** signatures *****)
 Inductive expr : Type :=
   | intl : nat -> expr
   | plus : expr -> expr -> expr.
 
+Inductive ty : Type :=
+  | intty : ty.
+
+Inductive mult : Type :=
+  | one : mult
+  | zeroOrOne : mult
+  | oneOrMore : mult
+  | zeroOrMore : mult.
+
 Inductive val : Type :=
   | intv : nat -> val.
 
-Fixpoint eval (b : expr) : val :=
-  match b with
-  | intl n => intv n
-  | plus e1 e2 =>
-      let v1 := eval e1 in
-      let v2 := eval e2 in
-      match v1, v2 with
-      | intv n1, intv n2 => intv (n1 + n2)
-      end
+(***** type check *****)
+(* TODO: needs to be a partial function *)
+Fixpoint tc (e : expr) : ty :=
+  match e with
+  | intl _ => intty
+  | plus e1 e2 => 
+      let t1 := tc e1 in
+      let t2 := tc e2 in
+      intty
   end.
 
-Example test_bin_incr1 :
-eval (plus (intl 1) (intl 2)) = intv 3.
-Proof. simpl. reflexivity.
-Qed.
+Example test_tc_1 :
+tc (plus (intl 1) (intl 2)) = intty.
+Proof. simpl. reflexivity. Qed.
 
-(*
-Fixpoint cross_product
-(v1s : list val) (v2s : list val) : Vector 2 val :=
-  v1s.
-
-Fixpoint eval2 (b : expr) : list val :=
-  match b with
-  | intl n => cons (intv n) nil
-  | plus e1 e2 =>
-      let v1 := eval2 e1 in
-      let v2 := eval2 e2 in
-      match v1, v2 with
-      | intv n1, intv n2 => intv (n1 + n2)
-      end
+(***** multiplicity check *****)
+(* TODO: lattice as in NaBL2? or keep as function? *)
+Definition mult_crossproduct (m1 : mult) (m2 : mult) : mult :=
+  match m1, m2 with
+  | one       , m2         => m2
+  | m1        , one        => m1
+  | zeroOrOne , zeroOrOne  => zeroOrOne
+  | oneOrMore , oneOrMore  => oneOrMore
+  | _         , _          => zeroOrMore
   end.
-*)
+
+Fixpoint mc (e : expr) : mult :=
+  match e with
+  | intl _ => one
+  | plus e1 e2 =>
+      let m1 := mc e1 in
+      let m2 := mc e2 in
+      mult_crossproduct m1 m2
+  end.
+
+Example test_mc_1 :
+mc (plus (intl 1) (intl 2)) = one.
+Proof. simpl. reflexivity. Qed.
+
+(***** interpreter *****)
+Definition eval_plus (v : val * val) : val :=
+  match v with
+  | (intv n1, intv n2) => intv (n1 + n2)
+  end.
+
+Fixpoint eval (b : expr) : list val :=
+  match b with
+  | intl n => [(intv n)]
+  | plus e1 e2 =>
+      let v1 : list val       := eval e1 in
+      let v2 : list val       := eval e2 in
+      let vs : list (val*val) := list_crossproduct v1 v2 in
+      map eval_plus vs
+  end.
+
+Example test_eval_1 :
+eval (plus (intl 1) (intl 2)) = [intv 3].
+Proof. simpl. reflexivity. Qed.
